Intermediate/PS.v
@@ -25,40 +25,50 @@ Inductive state : Type :=
 | CC : context_state -> exec_state -> state
 with exec_state : Type := Normal | WentWrong.
 
-(* The split between program and context is represented by the domain of the
-   entrypoints map. *)
-Definition is_program_component G C := NMap.In C (genv_entrypoints G).
-Definition is_context_component G C := ~ is_program_component G C.
+Definition is_program_component G C := NMap.In C (genv_interface G).
+Definition is_context_component (ctx: Program.interface) C := NMap.In C ctx.
 
 Definition initial_state
-           (G: global_env)
-           (mainC: Component.id) (mainP: Procedure.id)
+           (p: program) (G: global_env) (ctx: Program.interface)
            (s: state) : Prop :=
   match s with
   | PC (gps, mem, regs, pc) =>
     (* the global protected stack is empty *)
     gps = [] /\
+    (* mem exaclty contains all components memories and it comes from the init routine *)
+    (forall C, is_program_component G C <-> NMap.In C mem) /\
+    (let '(m, _, _) := init_all p in mem = m) /\
+    (* the origin register (R_AUX2) is set to 1 (meaning external call) *)
+    (* the R_ONE register is set to 1 *)
+    (* the other registers are set to undef *)
+    regs = [Int 1; Undef; Undef; Undef; Int 1; Undef; Undef] /\
     (* the program counter is pointing to the start of the main procedure *)
-    EntryPoint.get mainC mainP (genv_entrypoints G) = Some (Pointer.block pc) /\
-    Pointer.component pc = mainC /\
-    Pointer.offset pc = 0 /\
-    (* each program component has its own memory *)
-    (forall C, is_program_component G C -> NMap.In C mem)
+    is_program_component G (Pointer.component pc) /\
+    Pointer.component pc = fst (prog_main p) /\
+    EntryPoint.get (fst (prog_main p)) (snd (prog_main p))
+                   (genv_entrypoints G) = Some (Pointer.block pc) /\
+    Pointer.offset pc = 0
   | CC (pgps, mem, C) execst =>
     (* the global protected stack is empty *)
     pgps = [] /\
-    (* the execution didn't go wrong *)
-    execst = Normal /\
+    (* mem exaclty contains all program components memories *)
+    (forall C, is_program_component G C <-> NMap.In C mem) /\
+    (let '(m, _, _) := init_all p in mem = m) /\
     (* the executing component is the main one *)
-    C = mainC /\
-    (* each program component has its own memory *)
-    (forall C, is_program_component G C -> NMap.In C mem)
+    is_context_component ctx C /\
+    C = fst (prog_main p) /\
+    (* the execution didn't go wrong *)
+    execst = Normal
   end.
 
+(* maybe check whether mem is sound and pc & C are in the program or the context *)
 Definition final_state (G: global_env) (s: state) (r: nat) : Prop :=
   match s with
-  | PC (gps, mem, regs, pc) => executing G pc IHalt
-  | CC (pgps, mem, C) execst => execst = Normal
+  | PC (gps, mem, regs, pc) =>
+    Register.get R_COM regs = Int r /\
+    executing G pc IHalt
+  | CC (pgps, mem, C) execst =>
+    execst = Normal
   end.
 
 Definition to_partial_frame pc frame : PartialPointer.t :=
@@ -92,26 +102,67 @@ Proof.
   rewrite Hprogturn. rewrite Hpstack. reflexivity.
 Qed.
 
-Inductive step (G : global_env) : state -> trace -> state -> Prop :=
+Inductive step (ctx: Program.interface) (G : global_env) : state -> trace -> state -> Prop :=
 | Program_Epsilon:
     forall G' pgps (mem mem' wmem wmem' : Memory.t) Cmem'
       (regs regs' : Register.t) (pc pc' : Pointer.t),
-      (* G' has the same interface as G, but it can contain more
-         information regarding procedures and entrypoints *)
-      genv_extension G' G ->
-      (* wmem contains mem *)
+
+      (* G' is an extension of G w.r.t. ctx *)
+      (* 1) the interface is G plus ctx *)
+      NMap.Equal (genv_interface G') (NMapExtra.update (genv_interface G) ctx) ->
+      (* 2) the procedures are the same of G plus some new ones for ctx *)
+      (forall C Cprocs, NMap.MapsTo C Cprocs (genv_procedures G') <->
+                   (NMap.MapsTo C Cprocs (genv_procedures G) \/
+                    (NMap.In C ctx /\ ~ NMap.In C (genv_procedures G)))) ->
+      (* 3) the entrypoints are the same of G plus some new ones for ctx *)
+      (forall C Centrypoints, NMap.MapsTo C Centrypoints (genv_entrypoints G') <->
+                         (NMap.MapsTo C Centrypoints (genv_entrypoints G) \/
+                          (NMap.In C ctx /\ ~ NMap.In C (genv_entrypoints G)))) ->
+
+      (* wmem is an extension of mem w.r.t. ctx *)
+      (* 1) wmem contains mem *)
       (forall C Cmem, NMap.MapsTo C Cmem mem -> NMap.MapsTo C Cmem wmem) ->
-      (* wmem has the context components memories *)
-      (forall C, is_context_component G C -> NMap.In C wmem) ->
+      (* 2) wmem has the context components memories *)
+      (forall C, is_context_component ctx C -> NMap.In C wmem) ->
+      (* 3) wmem extends mem exactly w.r.t. ctx *)
+      (forall C Cmem, NMap.MapsTo C Cmem wmem <->
+                 (NMap.MapsTo C Cmem mem \/
+                  (is_context_component ctx C /\ ~ NMap.In C mem))) ->
+
       (* the complete semantics steps silently with the extended versions of
          memory and global environment
          NOTE that the stack (gps) is not related to the partial one (pgps) *)
       (exists gps, CS.step G' (gps,wmem,regs,pc) E0 (gps,wmem',regs',pc')) ->
+
       (* mem' is mem with the updated version of the current
          executing component's memory *)
-      NMap.MapsTo (Pointer.component pc) Cmem' wmem' ->
-      NMap.Equal mem' (NMap.add (Pointer.component pc) Cmem' mem) ->
-      step G (PC (pgps,mem,regs,pc)) E0 (PC (pgps,mem',regs',pc'))
+      NMap.MapsTo (Pointer.component pc') Cmem' wmem' ->
+      NMap.Equal mem' (NMap.add (Pointer.component pc') Cmem' mem) ->
+
+      step ctx G (PC (pgps,mem,regs,pc)) E0 (PC (pgps,mem',regs',pc'))
+
+| Program_External_Load_In_Program:
+    forall pgps mem regs regs' pc r1 r2 ptr v,
+      executing G pc (ILoad r1 r2) ->
+      Register.get r1 regs = Ptr ptr ->
+      Pointer.component ptr <> Pointer.component pc ->
+      is_program_component G (Pointer.component ptr) ->
+      Memory.load mem ptr = Some v ->
+      Register.set r2 v regs = regs' ->
+      (* TODO fix the read value in the event *)
+      let t := [ELoad (Pointer.component pc) 0 (Pointer.component ptr)] in
+      step ctx G (PC (pgps, mem, regs, pc)) t (PC (pgps, mem, regs', Pointer.inc pc))
+
+| Program_External_Load_In_Context:
+    forall pgps mem regs regs' pc r1 r2 ptr v,
+      executing G pc (ILoad r1 r2) ->
+      Register.get r1 regs = Ptr ptr ->
+      Pointer.component ptr <> Pointer.component pc ->
+      is_context_component ctx (Pointer.component ptr) ->
+      Register.set r2 v regs = regs' ->
+      (* TODO fix the read value in the event *)
+      let t := [ELoad (Pointer.component pc) 0 (Pointer.component ptr)] in
+      step ctx G (PC (pgps, mem, regs, pc)) t (PC (pgps, mem, regs', Pointer.inc pc))
 
 | Program_Internal_Call:
     forall pgps pgps' mem regs b o pc C' P val,
@@ -125,7 +176,7 @@ Inductive step (G : global_env) : state -> trace -> state -> Prop :=
       Register.get R_COM regs = Int val ->
       let pc' := (C', b, 0) in
       let t := [ECall C P val C'] in
-      step G (PC (pgps,mem,regs,pc)) t (PC (pgps',mem,Register.invalidate regs,pc'))
+      step ctx G (PC (pgps,mem,regs,pc)) t (PC (pgps',mem,Register.invalidate regs,pc'))
 
 | Program_Internal_Return:
     forall pgps pgps' mem regs pc pc' C' b o val,
@@ -136,7 +187,7 @@ Inductive step (G : global_env) : state -> trace -> state -> Prop :=
       is_program_component G C' ->
       Register.get R_COM regs = Int val ->
       let t := [ERet C val C'] in
-      step G (PC (pgps,mem,regs,pc)) t (PC (pgps',mem,Register.invalidate regs,pc'))
+      step ctx G (PC (pgps,mem,regs,pc)) t (PC (pgps',mem,Register.invalidate regs,pc'))
 
 | Program_External_Call:
     forall pgps pgps' mem regs pc C' b o P val,
@@ -144,60 +195,78 @@ Inductive step (G : global_env) : state -> trace -> state -> Prop :=
       executing G pc (ICall C' P) ->
       C' <> C ->
       imported_procedure (genv_interface G) C C' P ->
-      is_context_component G C' ->
+      is_context_component ctx C' ->
       pgps' = (C, Some (b,o)) :: pgps ->
       Register.get R_COM regs = Int val ->
+      (* TODO fix the read value in the event *)
       let t := [ECall C P val C'] in
-      step G (PC (pgps,mem,regs,pc)) t (CC (pgps',mem,C') Normal)
+      step ctx G (PC (pgps,mem,regs,pc)) t (CC (pgps',mem,C') Normal)
 
 | Program_External_Return:
     forall pgps pgps' mem regs pc C' val,
       let C := Pointer.component pc in
       executing G pc IReturn ->
       C' <> C ->
-      is_context_component G C' ->
+      is_context_component ctx C' ->
       pgps = (C', None) :: pgps' ->
       Register.get R_COM regs = Int val ->
+      (* TODO fix the read value in the event *)
       let t := [ERet C val C'] in
-      step G (PC (pgps,mem,regs,pc)) t (CC (pgps',mem,C') Normal)
+      step ctx G (PC (pgps,mem,regs,pc)) t (CC (pgps',mem,C') Normal)
 
 | Context_Epsilon:
     forall pgps mem C,
-      step G (CC (pgps,mem,C) Normal) E0 (CC (pgps,mem,C) Normal)
+      step ctx G (CC (pgps,mem,C) Normal) E0 (CC (pgps,mem,C) Normal)
 
 | Context_GoesWrong:
     forall pgps mem C,
-      step G (CC (pgps,mem,C) Normal) E0 (CC (pgps,mem,C) WentWrong)
+      step ctx G (CC (pgps,mem,C) Normal) E0 (CC (pgps,mem,C) WentWrong)
 
 | Context_Internal_Call:
     forall pgps pgps' mem C C' P call_arg,
       C' <> C ->
-      imported_procedure (genv_interface G) C C' P ->
-      is_context_component G C' ->
+      imported_procedure ctx C C' P ->
+      is_context_component ctx C' ->
       pgps' = (C, None) :: pgps ->
       let t := [ECall C P call_arg C'] in
-      step G (CC (pgps,mem,C) Normal) t (CC (pgps',mem,C') Normal)
+      step ctx G (CC (pgps,mem,C) Normal) t (CC (pgps',mem,C') Normal)
 
 | Context_Internal_Return:
     forall pgps pgps' mem C C' return_val,
       C' <> C ->
-      is_context_component G C' ->
+      is_context_component ctx C' ->
       pgps = (C', None) :: pgps' ->
       let t := [ERet C return_val C'] in
-      step G (CC (pgps,mem,C) Normal) t (CC (pgps',mem,C') Normal)
+      step ctx G (CC (pgps,mem,C) Normal) t (CC (pgps',mem,C') Normal)
+
+| Context_External_Load_In_Context:
+    forall pgps mem C ptr,
+      Pointer.component ptr <> C ->
+      is_context_component ctx (Pointer.component ptr) ->
+      (* TODO fix the read value in the event *)
+      let t := [ELoad C 0 (Pointer.component ptr)] in
+      step ctx G (CC (pgps, mem, C) Normal) t (CC (pgps, mem, C) Normal)
+
+| Context_External_Load_In_Program:
+    forall pgps mem C ptr v,
+      Pointer.component ptr <> C ->
+      is_program_component G (Pointer.component ptr) ->
+      Memory.load mem ptr = Some v ->
+      (* TODO fix the read value in the event *)
+      let t := [ELoad C 0 (Pointer.component ptr)] in
+      step ctx G (CC (pgps, mem, C) Normal) t (CC (pgps, mem, C) Normal)
 
 | Context_External_Call:
     forall pgps pgps' mem regs C C' P b val,
       C' <> C ->
-      exported_procedure (genv_interface G) C' P ->
-      imported_procedure (genv_interface G) C C' P ->
+      imported_procedure ctx C C' P ->
       is_program_component G C' ->
       pgps' = (C, None) :: pgps ->
       EntryPoint.get C' P (genv_entrypoints G) = Some b ->
       Register.get R_COM regs = Int val ->
       let t := [ECall C P val C'] in
       let pc' := (C', b, 0) in
-      step G (CC (pgps,mem,C) Normal) t (PC (pgps',mem,regs,pc'))
+      step ctx G (CC (pgps,mem,C) Normal) t (PC (pgps',mem,regs,pc'))
 
 | Context_External_Return:
     forall pgps pgps' mem regs C C' b o val,
@@ -205,44 +274,36 @@ Inductive step (G : global_env) : state -> trace -> state -> Prop :=
       is_program_component G C' ->
       Register.get R_COM regs = Int val ->
       let t := [ERet C val C'] in
-      step G (CC (pgps,mem,C) Normal) t (PC (pgps',mem,regs, (C',b,o))).
+      step ctx G (CC (pgps,mem,C) Normal) t (PC (pgps',mem,regs, (C',b,o))).
 
-Definition partialize (p: program) (ctx: Program.interface)
-           (mainC: Component.id) (mainP: Procedure.id)
-  : program :=
-  {| prog_interface := NMapExtra.update (prog_interface p) ctx;
-     prog_procedures := prog_procedures p;
-     prog_buffers := prog_buffers p;
-     prog_main := (mainC, mainP) |}.
+Definition partialize (p: program) (ctx: Program.interface) : program :=
+  {| prog_interface :=
+       NMapExtra.diff (prog_interface p) ctx;
+     prog_procedures :=
+       NMapExtra.filter (fun k _ => negb (NMap.mem k ctx)) (prog_procedures p);
+     prog_buffers :=
+       NMapExtra.filter (fun k _ => negb (NMap.mem k ctx)) (prog_buffers p);
+     prog_main := prog_main p |}.
 
 Section Semantics.
   Variable p: program.
-  Variable mainC: Component.id.
-  Variable mainP: Procedure.id.
-  Variable context_interface : Program.interface.
+  Variable ctx: Program.interface.
 
-  Definition partial_program := partialize p context_interface mainC mainP.
+  Let G := init_genv (partialize p ctx).
 
-  Let G := init_genv partial_program.
+  Hypothesis valid_program:
+    well_formed_program p.
+
+  Hypothesis complete_program:
+    closed_program p.
+
+  (* the context is part of p *)
+  Hypothesis valid_context:
+    forall C CI, NMap.MapsTo C CI ctx -> NMap.MapsTo C CI (prog_interface p).
 
   Definition sem :=
-    @Semantics_gen state global_env step
-                   (initial_state G (fst (prog_main partial_program))
-                                    (snd (prog_main partial_program)))
+    @Semantics_gen state global_env (step ctx)
+                   (initial_state (partialize p ctx) G ctx)
                    (final_state G) G.
 End Semantics.
-
-Definition maps_match_on {T : Type} split (map map' : NMap.t T) :=
-  forall C Cmap,
-    In C split ->
-    (NMap.MapsTo C Cmap map <-> NMap.MapsTo C Cmap map').
-
-Lemma maps_match_on_reflexive:
-  forall T split (mem: NMap.t T),
-    maps_match_on split mem mem.
-Proof.
-  unfold maps_match_on. intros.
-  split; auto.
-Qed.
-
 End PS.
