Source/Language.v
@@ -52,34 +52,67 @@ Module Source.
                    NMap.In P' C'procs))
     end.
 
-  (* Each component must have its own buffer of size at least one *)
+  (* Component C has a buffer of size at least one *)
   Definition has_required_local_buffers (p: program) (C: Component.id) : Prop :=
     exists size, NMap.find C (prog_buffers p) = Some size /\
             size > 0.
 
   Record well_formed_program (p: program) := {
+    (* the interface is sound (but maybe not closed) *)
     wfprog_interface_soundness:
       sound_interface (prog_interface p);
+    (* each declared components has the required static buffers *)
     wfprog_buffers_existence:
-      forall C, NMap.In C (prog_interface p) -> has_required_local_buffers p C;
+      forall C, NMap.In C (prog_interface p) ->
+           has_required_local_buffers p C;
+    (* each exported procedures actually exists *)
     wfprog_exported_procedures_existence:
       forall C CI,
         NMap.MapsTo C CI (prog_interface p) ->
       forall P,
         Component.is_exporting CI P ->
-      exists Cprocs Pexpr,
+      exists Cprocs,
         NMap.MapsTo C Cprocs (prog_procedures p) /\
-        NMap.MapsTo P Pexpr Cprocs;
-    wfprog_main_existence:
-      exists procs,
-        NMap.MapsTo (fst (prog_main p)) procs (prog_procedures p) /\
-        NMap.In (snd (prog_main p)) procs;
+        NMap.In P Cprocs;
+    (* each instruction of each procedure is well-formed *)
     wfprog_well_formed_procedures:
       forall C Cprocs P Pexpr,
         NMap.MapsTo C Cprocs (prog_procedures p) ->
         NMap.MapsTo P Pexpr Cprocs ->
-        well_formed_expr p C Pexpr
+        well_formed_expr p C Pexpr;
+    (* if the main component exists, then the main procedure must exist as well *)
+    wfprog_main_existence:
+      forall main_procs,
+        NMap.MapsTo (fst (prog_main p)) main_procs (prog_procedures p) ->
+        NMap.In (snd (prog_main p)) main_procs
   }.
+
+  (* a closed program is a program with a closed interface and an existing main
+     procedure *)
+  Record closed_program (p: program) := {
+    (* the interface must be closed (and consequently sound) *)
+    cprog_closed_interface:
+      closed_interface (prog_interface p);
+    (* the main procedure must exist *)
+    cprog_main_existence:
+      exists procs,
+        NMap.MapsTo (fst (prog_main p)) procs (prog_procedures p) /\
+        NMap.In (snd (prog_main p)) procs;
+  }.
+
+  Definition linkable_programs (p1 p2: program) : Prop :=
+    (* both programs are well-formed *)
+    well_formed_program p1 /\ well_formed_program p2 /\
+    (* their interfaces are disjoint *)
+    NMapExtra.Disjoint (prog_interface p1) (prog_interface p2) /\
+    (* the union of their interfaces is sound *)
+    sound_interface (NMapExtra.update (prog_interface p1) (prog_interface p2)).
+
+  Definition program_link (p1 p2: program) mainC mainP : program :=
+    {| prog_interface := NMapExtra.update (prog_interface p1) (prog_interface p2);
+       prog_procedures := NMapExtra.update (prog_procedures p1) (prog_procedures p2);
+       prog_buffers := NMapExtra.update (prog_buffers p1) (prog_buffers p2);
+       prog_main := (mainC, mainP) |}.
 
   Fixpoint alloc_buffers
            (bufs: list (Component.id * nat))
