Source/PS.v
@@ -22,63 +22,102 @@ Inductive state : Type :=
 | CC : context_state -> exec_state -> state
 with exec_state : Type := Normal | WentWrong.
 
-Definition initial_state
-           (G: global_env)
-           (mainC: Component.id) (mainP: Procedure.id)
-           (st: state) : Prop :=
+Definition initial_state (p: program) (st: state) : Prop :=
   match st with
   | PC (C, s, mem, k, e) =>
     (* the executing component is the main one *)
-    C = mainC /\
+    C = fst (prog_main p) /\
     (* the stack is empty *)
     s = [] /\
+    (* mem exaclty contains all components memories and it comes from the init routine *)
+    (forall C, NMap.In C (prog_interface p) <-> NMap.In C mem) /\
+    (let '(_, m) := init_all p in mem = m) /\
     (* the expression under evaluation is the main procedure *)
     (exists main_procs,
-        NMap.find mainC (genv_procedures G) = Some main_procs /\
-        NMap.find mainP main_procs = Some e) /\
+        NMap.find (fst (prog_main p)) (prog_procedures p) = Some main_procs /\
+        NMap.find (snd (prog_main p)) main_procs = Some e) /\
     (* the continuation is stop *)
     k = Kstop
   | CC (C, s, mem) execst =>
     (* the executing component is the main one *)
-    C = mainC /\
+    C = fst (prog_main p) /\
     (* the stack is empty *)
     s = [] /\
+    (* mem exaclty contains all components memories and it comes from the init routine *)
+    (forall C, NMap.In C (prog_interface p) <-> NMap.In C mem) /\
+    (let '(_, m) := init_all p in mem = m) /\
     (* the execution didn't go wrong *)
     execst = Normal
   end.
 
-Definition final_state (G: global_env) (st: state) (r: nat) : Prop :=
+Definition final_state (st: state) (r: nat) : Prop :=
   match st with
   | PC (C, s, mem, k, e) =>
-    e = E_exit /\ k = Kstop
+    e = E_exit
   | CC (C, s, mem) execst =>
     execst = Normal
   end.
 
-(* The split between program and context is represented by the domain of the
-   procedures map. *)
-Definition is_program_component G C := NMap.In C (genv_procedures G).
-Definition is_context_component G C := ~ is_program_component G C.
+Definition is_program_component G C := NMap.In C (genv_interface G).
+Definition is_context_component (ctx: Program.interface) C := NMap.In C ctx.
 
-Inductive kstep (G: global_env) : state -> trace -> state -> Prop :=
+Inductive kstep (ctx: Program.interface) (G: global_env) : state -> trace -> state -> Prop :=
 | Program_Epsilon:
     forall G' C s mem mem' Cmem' wmem wmem' k k' e e',
-      (* G' has the same interface as G, but it can contain more
-         information regarding procedures and entrypoints *)
-      genv_extension G' G ->
-      (* wmem contains mem *)
-      (forall C' C'mem, NMap.MapsTo C' C'mem mem -> NMap.MapsTo C' C'mem wmem) ->
-      (* wmem has the context components memories *)
-      (forall C, is_context_component G C -> NMap.In C wmem) ->
+      (* G' is an extension of G w.r.t. ctx *)
+      (* 1) the interface is G plus ctx *)
+      NMap.Equal (genv_interface G') (NMapExtra.update (genv_interface G) ctx) ->
+      (* 2) the procedures are the same of G plus some new ones for ctx *)
+      (forall C Cprocs, NMap.MapsTo C Cprocs (genv_procedures G') <->
+                   (NMap.MapsTo C Cprocs (genv_procedures G) \/
+                    (NMap.In C ctx /\ ~ NMap.In C (genv_procedures G)))) ->
+      (* 3) the buffers are the same of G plus some new ones for ctx *)
+      (forall C Cbufs, NMap.MapsTo C Cbufs (genv_buffers G') <->
+                  (NMap.MapsTo C Cbufs (genv_buffers G) \/
+                   (NMap.In C ctx /\ ~ NMap.In C (genv_buffers G)))) ->
+
+      (* wmem is an extension of mem w.r.t. ctx *)
+      (* 1) wmem contains mem *)
+      (forall C Cmem, NMap.MapsTo C Cmem mem -> NMap.MapsTo C Cmem wmem) ->
+      (* 2) wmem has the context components memories *)
+      (forall C, is_context_component ctx C -> NMap.In C wmem) ->
+      (* 3) wmem extends mem exactly w.r.t. ctx *)
+      (forall C Cmem, NMap.MapsTo C Cmem wmem <->
+                 (NMap.MapsTo C Cmem mem \/
+                  (is_context_component ctx C /\ ~ NMap.In C mem))) ->
+
       (* the complete semantics steps silently with the extended versions of
          memory and global environment
-         NOTE that the stack (gps) is not related to the partial one (pgps) *)
-      (exists s', CS.kstep G (C,s',wmem,k,e) E0 (C,s',wmem',k',e')) ->
+         NOTE that the stack (s) is not related to the partial one (ps) *)
+      (exists ps, CS.kstep G' (C,ps,wmem,k,e) E0 (C,ps,wmem',k',e')) ->
+
       (* mem' is mem with the updated version of the current
          executing component's memory *)
       NMap.MapsTo C Cmem' wmem' ->
       NMap.Equal mem' (NMap.add C Cmem' mem) ->
-      kstep G (PC (C,s,mem,k,e)) E0 (PC (C,s,mem',k',e'))
+
+      kstep ctx G (PC (C,s,mem,k,e)) E0 (PC (C,s,mem',k',e'))
+
+| Program_External_Load_In_Program:
+    forall C s mem k ptr v,
+      Pointer.component ptr <> C ->
+      is_program_component G (Pointer.component ptr) ->
+      Memory.load mem ptr = Some v ->
+      (* TODO fix the read value in the event *)
+      let t := [ELoad C 0 (Pointer.component ptr)] in
+      kstep ctx G
+            (PC (C, s, mem, Kderef k, E_val (Ptr ptr))) t
+            (PC (C, s, mem, k, E_val v))
+
+| Program_External_Load_In_Context:
+    forall C s mem k ptr v,
+      Pointer.component ptr <> C ->
+      is_context_component ctx (Pointer.component ptr) ->
+      (* TODO fix the read value in the event *)
+      let t := [ELoad C 0 (Pointer.component ptr)] in
+      kstep ctx G
+            (PC (C, s, mem, Kderef k, E_val (Ptr ptr))) t
+            (PC (C, s, mem, k, E_val v))
 
 | Program_Internal_Call:
     forall C s mem mem' k C' P v C'_procs P_expr b b' old_call_arg,
@@ -93,8 +132,9 @@ Inductive kstep (G: global_env) : state -> trace -> state -> Prop :=
       NMap.find C' (genv_buffers G) = Some b' ->
       Memory.store mem (C',b',0) (Int v) = Some mem' ->
       let t := if C =? C' then E0 else [ECall C P v C'] in
-      kstep G (PC (C, s, mem, Kcall C' P k, E_val (Int v)))
-            t (PC (C', (C, Some (old_call_arg, k)) :: s, mem', Kstop, P_expr))
+      kstep ctx G
+            (PC (C, s, mem, Kcall C' P k, E_val (Int v))) t
+            (PC (C', (C, Some (old_call_arg, k)) :: s, mem', Kstop, P_expr))
 
 | Program_Internal_Return:
     forall C s mem mem' k v C' old_call_arg b,
@@ -103,50 +143,70 @@ Inductive kstep (G: global_env) : state -> trace -> state -> Prop :=
       NMap.find C' (genv_buffers G) = Some b ->
       Memory.store mem (C', b, 0) old_call_arg = Some mem' ->
       let t := if C =? C' then E0 else [ERet C v C'] in
-      kstep G (PC (C, (C', Some (old_call_arg, k)) :: s, mem, Kstop, E_val (Int v)))
-            t (PC (C', s, mem', k, E_val (Int v)))
+      kstep ctx G
+            (PC (C, (C', Some (old_call_arg, k)) :: s, mem, Kstop, E_val (Int v))) t
+            (PC (C', s, mem', k, E_val (Int v)))
 
 | Program_External_Call:
     forall C s mem k C' P v b old_call_arg,
-      is_context_component G C' ->
+      is_context_component ctx C' ->
       (* save the old call argument *)
       NMap.find C (genv_buffers G) = Some b ->
       Memory.load mem (C,b,0) = Some old_call_arg ->
       let t := [ECall C P v C'] in
-      kstep G (PC (C, s, mem, Kcall C' P k, E_val (Int v)))
-            t (CC (C', (C, Some (old_call_arg,k)) :: s, mem) Normal)
+      kstep ctx G
+            (PC (C, s, mem, Kcall C' P k, E_val (Int v))) t
+            (CC (C', (C, Some (old_call_arg,k)) :: s, mem) Normal)
 
 | Program_External_Return:
     forall C s mem k v C' old_call_arg,
-      is_context_component G C' ->
+      is_context_component ctx C' ->
       let t := [ERet C v C'] in
-      kstep G (PC (C, (C', Some (old_call_arg, k)) :: s, mem, Kstop, E_val (Int v)))
-            t (CC (C', s, mem) Normal)
+      kstep ctx G
+            (PC (C, (C', Some (old_call_arg, k)) :: s, mem, Kstop, E_val (Int v))) t
+            (CC (C', s, mem) Normal)
 
 | Context_Epsilon:
     forall s mem C,
-      kstep G (CC (C,s,mem) Normal) E0 (CC (C,s,mem) Normal)
+      kstep ctx G (CC (C,s,mem) Normal) E0 (CC (C,s,mem) Normal)
 
 | Context_GoesWrong:
     forall s mem C,
-      kstep G (CC (C,s,mem) Normal) E0 (CC (C,s,mem) WentWrong)
+      kstep ctx G (CC (C,s,mem) Normal) E0 (CC (C,s,mem) WentWrong)
+
+| Context_External_Load_In_Context:
+    forall s mem C ptr,
+      Pointer.component ptr <> C ->
+      is_context_component ctx (Pointer.component ptr) ->
+      (* TODO fix the read value in the event *)
+      let t := [ELoad C 0 (Pointer.component ptr)] in
+      kstep ctx G (CC (C,s,mem) Normal) t (CC (C, s, mem) Normal)
+
+| Context_External_Load_In_Program:
+    forall s mem C ptr v,
+      Pointer.component ptr <> C ->
+      is_program_component G (Pointer.component ptr) ->
+      Memory.load mem ptr = Some v ->
+      (* TODO fix the read value in the event *)
+      let t := [ELoad C 0 (Pointer.component ptr)] in
+      kstep ctx G (CC (C, s, mem) Normal) t (CC (C, s, mem) Normal)
 
 | Context_Internal_Call:
     forall s s' mem C C' P call_arg,
       C' <> C ->
       imported_procedure (genv_interface G) C C' P ->
-      is_context_component G C' ->
+      is_context_component ctx C' ->
       s' = (C, None) :: s ->
       let t := [ECall C P call_arg C'] in
-      kstep G (CC (C,s,mem) Normal) t (CC (C',s',mem) Normal)
+      kstep ctx G (CC (C,s,mem) Normal) t (CC (C',s',mem) Normal)
 
 | Context_Internal_Return:
     forall s s' mem C C' return_val,
       C' <> C ->
-      is_context_component G C' ->
+      is_context_component ctx C' ->
       s = (C', None) :: s' ->
       let t := [ERet C return_val C'] in
-      kstep G (CC (C,s,mem) Normal) t (CC (C',s',mem) Normal)
+      kstep ctx G (CC (C,s,mem) Normal) t (CC (C',s',mem) Normal)
 
 | Context_External_Call:
     forall s s' mem mem' C C' P C'_procs P_expr b' val,
@@ -162,7 +222,7 @@ Inductive kstep (G: global_env) : state -> trace -> state -> Prop :=
       NMap.find C' (genv_buffers G) = Some b' ->
       Memory.store mem (C',b',0) (Int val) = Some mem' ->
       let t := [ECall C P val C'] in
-      kstep G (CC (C,s,mem) Normal) t (PC (C',s',mem,Kstop,P_expr))
+      kstep ctx G (CC (C,s,mem) Normal) t (PC (C',s',mem,Kstop,P_expr))
 
 | Context_External_Return:
     forall C s mem mem' k v C' old_call_arg b,
@@ -170,12 +230,14 @@ Inductive kstep (G: global_env) : state -> trace -> state -> Prop :=
       (* restore the old call argument *)
       NMap.find C' (genv_buffers G) = Some b ->
       Memory.store mem (C', b, 0) old_call_arg = Some mem' ->
-      let t := [ERet C v C']in
-      kstep G (CC (C, (C', Some (old_call_arg, k)) :: s, mem) Normal)
-            t (PC (C', s, mem', k, E_val (Int v))).
+      let t := [ERet C v C'] in
+      kstep ctx G
+            (CC (C, (C', Some (old_call_arg, k)) :: s, mem) Normal) t
+            (PC (C', s, mem', k, E_val (Int v))).
 
 Definition partialize (p: program) (ctx: Program.interface) : program :=
-  {| prog_interface := prog_interface p;
+  {| prog_interface :=
+       NMapExtra.diff (prog_interface p) ctx;
      prog_procedures :=
        NMapExtra.filter (fun C _ => negb (NMap.mem C ctx)) (prog_procedures p);
      prog_buffers :=
@@ -184,15 +246,22 @@ Definition partialize (p: program) (ctx: Program.interface) : program :=
 
 Section Semantics.
   Variable p: program.
-  Variable context_interface : Program.interface.
+  Variable ctx: Program.interface.
 
-  Definition partial_program := partialize p context_interface.
-  Let G := init_genv partial_program.
+  Let G := init_genv (partialize p ctx).
+
+  Hypothesis valid_program:
+    well_formed_program p.
+
+  Hypothesis complete_program:
+    closed_program p.
+
+  (* the context is part of p *)
+  Hypothesis valid_context:
+    forall C CI, NMap.MapsTo C CI ctx -> NMap.MapsTo C CI (prog_interface p).
 
   Definition sem :=
-    @Semantics_gen state global_env kstep
-                   (initial_state G (fst (prog_main p)) (snd (prog_main p)))
-                   (final_state G) G.
+    @Semantics_gen state global_env (kstep ctx)
+                   (initial_state (partialize p ctx)) final_state G.
 End Semantics.
-
 End PS.
