Common/Linking.v
@@ -22,6 +22,21 @@ Definition closed_interface (interface : Program.interface) : Prop :=
     Program.has_component interface C' CI' /\
     Component.is_exporting CI' P.
 
+Lemma closed_interface_is_sound:
+  forall iface,
+    closed_interface iface -> sound_interface iface.
+Proof.
+  unfold closed_interface, sound_interface.
+  intros iface Hiface_closed.
+  intros.
+  specialize (Hiface_closed C CI H C' P H0).
+  destruct Hiface_closed as [CI'' [H1' H2]].
+  unfold Program.has_component in H1, H1'.
+  enough (HsameCI: CI' = CI'').
+  - subst. auto.
+  - apply NMapExtra.F.MapsTo_fun with iface C'; auto.
+Qed.
+
 Definition mergeable_interfaces (i1 i2 : Program.interface) : Prop :=
   NMapExtra.Disjoint i1 i2.
 
