Source/Definability.v
@@ -1,0 +1,29 @@
+Require Import Common.Definitions.
+Require Import Common.Util.
+Require Import Common.Values.
+Require Import Common.Memory.
+Require Import CompCert.Events.
+Require Import CompCert.Smallstep.
+Require Import CompCert.Behaviors.
+Require Import Source.Language.
+Require Import Source.GlobalEnv.
+Require Import Source.CS.
+Require Import Source.PS.
+
+Import Source.
+
+Section Definability.
+  Variable p: program.
+  Variable ictx: Program.interface.
+  Variable mainC: Component.id.
+  Variable mainP: Procedure.id.
+
+  Theorem context_definability:
+    forall beh,
+      program_behaves (PS.sem p ictx) beh ->
+    exists ctx,
+      NMap.Equal (prog_interface ctx) ictx /\
+      program_behaves (CS.sem (program_link p ctx mainC mainP)) beh.
+  Proof.
+  Admitted.
+End Definability.
